% This is part of Analyse Starter CTU
% Copyright (c) 2016
%   Laurent Claessens,Carlotta Donadello
% See the file fdl-1.3.txt for copying conditions.

\begin{corrige}{analyseCTU-0109}
 
   \begin{enumerate}
   \item 
     \begin{equation*}
       \lim_{x\to 0}\left(\frac{1+\sin (x)-\cos(x)}{1-\sin (x)-\cos(x)}\right) = \lim_{x\to 0} \frac{1+x-1}{1-x-1} =-1\:;
     \end{equation*}
    \item 
      \begin{equation*}
        \lim_{x\to 0}\left(\frac{(1-\cos(3x))^2}{x^2(1-\cos(x))}\right) = \lim_{x\to 0} \frac{\left((1-1+\frac{(3x)^2}{2}\right)^2}{x^2\left(1-1+\frac{x^2}{2}\right)} = \frac{81}{2} \:;
      \end{equation*}
    \item 
      \begin{equation*}
        \lim_{x\to 0}\left(\frac{\sin (5x)}{\ln(1+4x)}\right)=\lim_{x\to 0}\frac{5x }{4x} = \frac{5}{4}.
      \end{equation*}
   \end{enumerate}


\end{corrige}
